Added checkers for UniqueBinders.v

src/Language/PlutusIR/Analysis/UniqueBinders.v
@@ -5,95 +5,116 @@ Require Import PlutusCert.Language.PlutusIR.Analysis.BoundVars.
 Require Import PlutusCert.Language.PlutusIR.Semantics.Static.
 Require Import PlutusCert.Util.
 
-Require Import Coq.Lists.List.
+Import Coq.Lists.List.
+Import Coq.Strings.String.
+Local Open Scope string_scope.
 
-Module Ty.
+From QuickChick Require Import QuickChick.
 
-  Inductive unique : Ty -> Prop :=
-    | UNI_TyFun : forall T1 T2,
-        unique T1 ->
-        unique T2 ->
-        unique (Ty_Fun T1 T2)
-    | UNI_TyBuiltin : forall st,
-        unique (Ty_Builtin st)
-    | UNI_TyVar : forall X,
-        unique (Ty_Var X)
-    | UNI_TyForall : forall X K T,
-        ~ Ty.appears_bound_in X T ->
-        unique T ->
-        unique (Ty_Forall X K T)
-    | UNI_TyIFix : forall F T,
-        unique F ->
-        unique T ->
-        unique (Ty_IFix F T)
-    | UNI_TyLam : forall X K T,
-        ~ Ty.appears_bound_in X T ->
-        unique T ->
-        unique (Ty_Lam X K T)
-    | UNI_TyApp : forall T1 T2,
-        unique T1 ->
-        unique T2 ->
-        unique (Ty_App T1 T2)
-    .
+Inductive unique_ty : Ty -> Prop :=
+  | UNI_TyFun : forall T1 T2,
+      unique_ty T1 ->
+      unique_ty T2 ->
+      unique_ty (Ty_Fun T1 T2)
+  | UNI_TyBuiltin : forall st,
+      unique_ty (Ty_Builtin st)
+  | UNI_TyVar : forall X,
+      unique_ty (Ty_Var X)
+  | UNI_TyForall : forall X K T,
+      ~ appears_bound_in_ty X T ->
+      unique_ty T ->
+      unique_ty (Ty_Forall X K T)
+  | UNI_TyIFix : forall F T,
+      unique_ty F ->
+      unique_ty T ->
+      unique_ty (Ty_IFix F T)
+  | UNI_TyLam : forall X K T,
+      ~ appears_bound_in_ty X T ->
+      unique_ty T ->
+      unique_ty (Ty_Lam X K T)
+  | UNI_TyApp : forall T1 T2,
+      unique_ty T1 ->
+      unique_ty T2 ->
+      unique_ty (Ty_App T1 T2)
+  .
 
-End Ty.
+QCDerive DecOpt for (unique_ty ty).
 
-Module Term.
+Instance unique_ty_DecOpt_sound ty : DecOptSoundPos (unique_ty ty).
+Proof. derive_sound. Qed.
 
-  Inductive unique : Term -> Prop :=
-    | UNI_Var : forall x,
-        unique (Var x)
-    | UNI_LamAbs : forall x T t,
-        ~ Term.appears_bound_in x t ->
-        unique t ->
-        Ty.unique T ->
-        unique (LamAbs x T t)
-    | UNI_App : forall t1 t2,
-        unique t1 ->
-        unique t2 ->
-        unique (Apply t1 t2)
-    | UNI_TyAbs : forall X K t,
-        ~ Annotation.appears_bound_in X t ->
-        unique t ->   
-        unique (TyAbs X K t)
-    | UNI_TyInst : forall t T,
-        unique t ->
-        Ty.unique T ->
-        unique (TyInst t T)
-    | UNI_IWrap : forall F T t,
-        Ty.unique F ->
-        Ty.unique T ->
-        unique t ->
-        unique (IWrap F T t)
-    | UNI_Unwrap : forall t,
-        unique t ->
-        unique (Unwrap t)
-    | UNI_Constant : forall sv,
-        unique (Constant sv)
-    | UNI_Builtin : forall f,
-        unique (Builtin f)
-    | UNI_Error : forall T,
-        Ty.unique T ->
-        unique (Error T)
-    | UNI_Let_Nil : forall recty t0,
-        unique t0 ->
-        unique (Let recty nil t0)
-    | UNI_Let_TermBind : forall recty stricty x T t bs t0,
-        ~ Term.appears_bound_in x t ->
-        ~ Term.appears_bound_in x (Let recty bs t0) ->
-        unique t ->
-        unique (Let recty bs t0) ->
-        unique (Let recty (TermBind stricty (VarDecl x T) t :: bs) t0)
-    | UNI_Let_TypeBind : forall recty X K T bs t0,
-        ~ Ty.appears_bound_in X T ->
-        ~ Annotation.appears_bound_in X (Let recty bs t0) ->
-        Ty.unique T ->
-        unique (Let recty bs t0) ->
-        unique (Let recty (TypeBind (TyVarDecl X K) T :: bs) t0)
-    | UNI_Let_DatatypeBind : forall recty X K YKs mfunc cs t0 bs,
-        ~ Annotation.appears_bound_in X (Let recty bs t0) ->
-        unique (Let recty bs t0) ->
-        unique (Let recty (DatatypeBind (Datatype (TyVarDecl X K) YKs mfunc cs) :: bs) t0) 
-    .
+(* FIXME: I don't think you can derive soundness for relations with negative constraints, unless you
+    proof a negative completeness proof for said constrain *)
+Instance unique_ty_DecOpt_complete ty : DecOptCompletePos (unique_ty ty).
+Proof. idtac "Admitted: unique_ty_decopt_complete". Admitted.
 
-End Term.
+Instance unique_ty_DecOpt_monotonic ty : DecOptSizeMonotonic (unique_ty ty).
+Proof. derive_mon. Qed.
+
+Inductive unique_tm : Term -> Prop :=
+  | UNI_Var : forall x,
+      unique_tm (Var x)
+  | UNI_LamAbs : forall x T t,
+      ~ appears_bound_in_tm x t ->
+      unique_tm t ->
+      unique_ty T ->
+      unique_tm (LamAbs x T t)
+  | UNI_App : forall t1 t2,
+      unique_tm t1 ->
+      unique_tm t2 ->
+      unique_tm (Apply t1 t2)
+  | UNI_TyAbs : forall X K t,
+      ~ appears_bound_in_ann X t ->
+      unique_tm t ->   
+      unique_tm (TyAbs X K t)
+  | UNI_TyInst : forall t T,
+      unique_tm t ->
+      unique_ty T ->
+      unique_tm (TyInst t T)
+  | UNI_IWrap : forall F T t,
+      unique_ty F ->
+      unique_ty T ->
+      unique_tm t ->
+      unique_tm (IWrap F T t)
+  | UNI_Unwrap : forall t,
+      unique_tm t ->
+      unique_tm (Unwrap t)
+  | UNI_Constant : forall sv,
+      unique_tm (Constant sv)
+  | UNI_Builtin : forall f,
+      unique_tm (Builtin f)
+  | UNI_Error : forall T,
+      unique_ty T ->
+      unique_tm (Error T)
+  | UNI_Let_Nil : forall recty t0,
+      unique_tm t0 ->
+      unique_tm (Let recty nil t0)
+  | UNI_Let_TermBind : forall recty stricty x T t bs t0,
+      ~ appears_bound_in_tm x t ->
+      ~ appears_bound_in_tm x (Let recty bs t0) ->
+      unique_tm t ->
+      unique_tm (Let recty bs t0) ->
+      unique_tm (Let recty (TermBind stricty (VarDecl x T) t :: bs) t0)
+  | UNI_Let_TypeBind : forall recty X K T bs t0,
+      ~ appears_bound_in_ty X T ->
+      ~ appears_bound_in_ann X (Let recty bs t0) ->
+      unique_ty T ->
+      unique_tm (Let recty bs t0) ->
+      unique_tm (Let recty (TypeBind (TyVarDecl X K) T :: bs) t0)
+  | UNI_Let_DatatypeBind : forall recty X K YKs mfunc cs t0 bs,
+      ~ appears_bound_in_ann X (Let recty bs t0) ->
+      unique_tm (Let recty bs t0) ->
+      unique_tm (Let recty (DatatypeBind (Datatype (TyVarDecl X K) YKs mfunc cs) :: bs) t0).
+
+QCDerive DecOpt for (unique_tm tm).
+
+Instance unique_tm_DecOpt_sound tm : DecOptSoundPos (unique_tm tm).
+Proof. derive_sound. Qed.
+
+(* FIXME: I don't think you can derive soundness for relations with negative constraints, unless you
+    proof a negative completeness proof for said constrain *)
+Instance unique_tm_DecOpt_complete tm : DecOptCompletePos (unique_tm tm).
+Proof. idtac "Admitted: unique_tm_DecOpt_complete". Admitted.
+
+Instance unique_tm_DecOpt_monotonic ty : DecOptSizeMonotonic (unique_ty ty).
+Proof. derive_mon. Qed.
